src/Example_proc.v
@@ -5,8 +5,8 @@ Definition val := T01 (Tint 16).
 
 Definition reg :=  T01 (Tint 2).  
 Definition RF := Tregfile 4 (val). 
-Definition instr : type1 := 
-  Tunion "instr" ("LOADI"  of (Ttuple [reg ;val]) 
+Definition INSTR : type1 := 
+  Tunion "INSTR" ("LOADI"  of (Ttuple [reg ;val]) 
                  :: "LOADPC" of (reg) 
                  :: "ADD" of (Ttuple [reg;reg;reg]) 
                  :: "BZ" of (Ttuple [reg;reg])
@@ -14,8 +14,8 @@ Definition instr : type1 :=
                  :: "STORE" of (Ttuple [reg;reg])
                  :: type1_id_list_nil ). 
 
-Definition IMEM := Tregfile (two_power_nat 16) instr. 
-Definition DMEM := Tregfile (two_power_nat 16) val. 
+Definition IMEM := Tregfile (128) INSTR. 
+Definition DMEM := Tregfile (128) val. 
 Definition PC := Treg val. 
 Definition state := [PC; RF; IMEM; DMEM]. 
 
@@ -37,59 +37,53 @@ Arguments WHERE {E F t} p%pattern e%expr.
 Notation "M  '[' ? key ']' " :=
 (Eget_regfile _ _ M _ key)(at level 0, no associativity) : expr_scope. 
 
-Definition IS_LOADI : pattern1 ([Treg reg ; Treg val]) instr.  
-apply Punion. apply pattern1_disjunct_hd. apply ( [| Pvar1 reg , Pvar1 val|])%pattern. 
-Defined. 
+Ltac case_match s :=
+let rec tac :=
+    match goal with 
+        |- pattern1_disjunct _ (type1_id_list_cons ?id ?t ?q) => 
+          first [(constr_eq s id; apply pattern1_disjunct_hd) 
+                | apply pattern1_disjunct_tl; tac]
+                
+    end
+in 
+  apply Punion;
+  tac; 
+try  match goal with 
+  |- pattern1 [?x] (?tv) => apply Pvar1
+  | |- pattern1 [?x1 ; ?x2] (Ttuple [?t1 ; ?t2]) => apply ([| Pvar1 _ , Pvar1 _|])%pattern
+  | |- pattern1 [?x1 ; ?x2 ; ?x3] (Ttuple [?t1 ; ?t2 ; ?t3]) => apply ([| Pvar1 _ , Pvar1 _ , Pvar1 _|])%pattern
+  end. 
 
-Definition IS_LOADPC : pattern1 ([Treg reg]) instr.  
-apply Punion. 
-apply pattern1_disjunct_tl. 
-apply pattern1_disjunct_hd. apply Pvar1. 
-Defined. 
+Definition IS_LOADI : pattern1 ([Treg reg ; Treg val]) INSTR.  
+case_match "LOADI". Defined. 
 
-Definition IS_ADD : pattern1 ([Treg reg; Treg reg; Treg reg]) instr.  
-apply Punion. 
-apply pattern1_disjunct_tl. 
-apply pattern1_disjunct_tl. 
-apply pattern1_disjunct_hd. apply ([| Pvar1 _ , Pvar1 _, Pvar1 _ |])%pattern. 
-Defined. 
+Definition IS_LOADPC : pattern1 ([Treg reg]) INSTR.  
+case_match "LOADPC". Defined. 
 
-Definition IS_BZ : pattern1 ([Treg reg; Treg reg]) instr.  
-apply Punion. 
-apply pattern1_disjunct_tl. 
-apply pattern1_disjunct_tl. 
-apply pattern1_disjunct_tl. 
-apply pattern1_disjunct_hd. apply ([| Pvar1 _ , Pvar1 _ |])%pattern. 
-Defined. 
+Definition IS_ADD : pattern1 ([Treg reg; Treg reg; Treg reg]) INSTR.  
+case_match "ADD". Defined. 
 
-Definition IS_LOAD : pattern1 ([Treg reg; Treg reg]) instr.  
-apply Punion. 
-apply pattern1_disjunct_tl. 
-apply pattern1_disjunct_tl. 
-apply pattern1_disjunct_tl. 
-apply pattern1_disjunct_tl. 
-apply pattern1_disjunct_hd. apply ([| Pvar1 _ , Pvar1 _ |])%pattern. 
-Defined. 
+Definition IS_BZ : pattern1 ([Treg reg; Treg reg]) INSTR.  
+case_match "BZ". Defined. 
 
-Definition IS_STORE : pattern1 ([Treg reg; Treg reg]) instr.  
-apply Punion. 
-apply pattern1_disjunct_tl. 
-apply pattern1_disjunct_tl. 
-apply pattern1_disjunct_tl. 
-apply pattern1_disjunct_tl. 
-apply pattern1_disjunct_tl. 
-apply pattern1_disjunct_hd. apply ([| Pvar1 _ , Pvar1 _ |])%pattern. 
-Defined. 
+Definition IS_LOAD : pattern1 ([Treg reg; Treg reg]) INSTR.  
+case_match "LOAD". Defined. 
+
+Definition IS_STORE : pattern1 ([Treg reg; Treg reg]) INSTR.  
+case_match "STORE". Defined. 
+
+Section rules. 
+
+Let env1 := state. 
+Let pc := var_0 : var env1 PC. 
+Let rf := var_S var_0 : var env1 RF. 
+Let imem := var_S (var_S var_0) : var env1 IMEM. 
+Let dmem := var_S (var_S (var_S var_0)) : var env1 DMEM. 
 
 (* (pc,rf,imem,dmem) where LOADI(rd,const) = imem[pc]
      –> (pc+1, rf[rd <- const], imem, dmem) *)
 Definition loadi_rule : rule state. 
-set (env1 := state). 
-set (env2 := List.app state  [Treg reg ; Treg val]). 
-set (pc := var_0 : var env1 PC). 
-set (rf := var_S var_0 : var env1 RF). 
-set (imem := var_S (var_S var_0) : var env1 IMEM). 
-set (dmem := var_S (var_S (var_S var_0)) : var env1 DMEM). 
+set (env2 := List.app env1  [Treg reg ; Treg val]). 
 set (rd := var_S (var_S (var_S (var_S var_0))) : var env2 (Treg reg)). 
 set (const := var_S (var_S (var_S (var_S (var_S var_0)))) : var env2 (Treg val)). 
 
@@ -107,12 +101,7 @@ Defined.
      –> (pc+1, rf[rd <- pc], imem, dmem) *)
 
 Definition loadpc_rule : rule state. 
-set (env1 := state). 
 set (env2 := List.app state  [Treg reg]). 
-set (pc := var_0 : var env1 PC). 
-set (rf := var_S var_0 : var env1 RF). 
-set (imem := var_S (var_S var_0) : var env1 IMEM). 
-set (dmem := var_S (var_S (var_S var_0)) : var env1 DMEM). 
 set (rd := var_S (var_S (var_S (var_S var_0))) : var env2 (Treg reg)). 
 
 apply (mk_rule state env1 env2). 
@@ -127,12 +116,7 @@ Defined.
 (* (pc,rf,imem,dmem) where ADD(rd,r1,r2) = imem[pc]
      –> (pc+1, rf[rd <- rf[r1] + rf[r2]], imem, dmem) *)
 Definition add_rule : rule state. 
-set (env1 := state). 
 set (env2 := List.app state  [Treg reg; Treg reg; Treg reg]). 
-set (pc := var_0 : var env1 PC). 
-set (rf := var_S var_0 : var env1 RF). 
-set (imem := var_S (var_S var_0) : var env1 IMEM). 
-set (dmem := var_S (var_S (var_S var_0)) : var env1 DMEM). 
 set (rd := var_S (var_S (var_S (var_S var_0))) : var env2 (Treg reg)). 
 set (r1 := var_S (var_S (var_S (var_S (var_S var_0)))) : var env2 (Treg reg)). 
 set (r2 := var_S (var_S (var_S (var_S (var_S (var_S var_0))))) : var env2 (Treg reg)). 
@@ -152,12 +136,7 @@ Defined.
 (* (pc,rf,imem,dmem) where BZ(rc,ra) = imem[pc] 
      –> (rf[ra], rf , imem, dmem) when rf[rc] = 0 *)
 Definition bztaken_rule : rule state. 
-set (env1 := state). 
 set (env2 := List.app state  [Treg reg; Treg reg]). 
-set (pc := var_0 : var env1 PC). 
-set (rf := var_S var_0 : var env1 RF). 
-set (imem := var_S (var_S var_0) : var env1 IMEM). 
-set (dmem := var_S (var_S (var_S var_0)) : var env1 DMEM). 
 set (rc := var_S (var_S (var_S (var_S var_0))) : var env2 (Treg reg)). 
 set (ra := var_S (var_S (var_S (var_S (var_S var_0)))) : var env2 (Treg reg)). 
 
@@ -175,12 +154,7 @@ Defined.
 (* (pc,rf,imem,dmem) where BZ(rc,ra) = imem[pc] 
      –> (pc+1, rf, imem, dmem) when rf[rc] <> 0 *)
 Definition bznottaken_rule : rule state. 
-set (env1 := state). 
 set (env2 := List.app state  [Treg reg; Treg reg]). 
-set (pc := var_0 : var env1 PC). 
-set (rf := var_S var_0 : var env1 RF). 
-set (imem := var_S (var_S var_0) : var env1 IMEM). 
-set (dmem := var_S (var_S (var_S var_0)) : var env1 DMEM). 
 set (rc := var_S (var_S (var_S (var_S var_0))) : var env2 (Treg reg)). 
 set (ra := var_S (var_S (var_S (var_S (var_S var_0)))) : var env2 (Treg reg)). 
 
@@ -198,12 +172,7 @@ Defined.
 (* (pc,rf,imem,dmem) where LOAD(rd,ra) = imem[pc] 
      –> (pc+1, rf[rd := dmem[rf [ra ]]], imem, dmem) *)
 Definition load_rule : rule state. 
-set (env1 := state). 
 set (env2 := List.app state  [Treg reg; Treg reg]). 
-set (pc := var_0 : var env1 PC). 
-set (rf := var_S var_0 : var env1 RF). 
-set (imem := var_S (var_S var_0) : var env1 IMEM). 
-set (dmem := var_S (var_S (var_S var_0)) : var env1 DMEM). 
 set (rd := var_S (var_S (var_S (var_S var_0))) : var env2 (Treg reg)). 
 set (ra := var_S (var_S (var_S (var_S (var_S var_0)))) : var env2 (Treg reg)). 
 
@@ -221,12 +190,7 @@ Defined.
 (* (pc,rf,imem,dmem) where STORE(ra,r) = imem[pc] 
      –> (pc+1, rf, imem, dmem[rf[ra] := rf[r]]) *)
 Definition store_rule : rule state. 
-set (env1 := state). 
 set (env2 := List.app state  [Treg reg; Treg reg]). 
-set (pc := var_0 : var env1 PC). 
-set (rf := var_S var_0 : var env1 RF). 
-set (imem := var_S (var_S var_0) : var env1 IMEM). 
-set (dmem := var_S (var_S (var_S var_0)) : var env1 DMEM). 
 set (ra := var_S (var_S (var_S (var_S var_0))) : var env2 (Treg reg)). 
 set (r := var_S (var_S (var_S (var_S (var_S var_0)))) : var env2 (Treg reg)). 
 
@@ -254,12 +218,78 @@ Definition TRS : TRS :=
                  store_rule
                ]|}. 
 
-Definition init : eval_env eval_type2 state.
-unfold eval_env. red. 
-split. simpl. apply (Word.repr _ 0). 
-split. simpl. apply Regfile.empty. apply (Word.repr _ 0).
-split. simpl eval_env. compute. 
-Definition AA : Word.T 32 := Word.repr 32 31. 
-Definition BB : Word.T 32 := Word.repr 32 3. 
-Admitted.     
+End rules. 
+
+Module Model. 
+  Inductive reg : Type := R1 | R2 | R3 | R4. 
+  Definition val := Word.T 16. 
+
+  Inductive instr :=
+    | loadi  : reg -> val -> instr
+    | loadpc : reg -> instr
+    | add : reg -> reg -> reg -> instr
+    | bz : reg -> reg -> instr
+    | load : reg -> reg -> instr
+    | store : reg -> reg -> instr. 
+
+  Record state :=
+    {
+      pc : val;
+      rf : reg -> val;
+      imem : val -> instr;        (* wrong *)
+      dmem : val -> val
+    }.
+End Model. 
+
+
+Class relate (X Y : Type) : Type := transform : (X -> Y).  
+Notation "X ==> Y" := (relate X Y) (at level 60). 
+Instance foo_reg : relate (Model.reg) (eval_type1 reg).  
+unfold relate;
+refine (fun x => match x with 
+                    | Model.R1 => Word.repr _ 0
+                    | Model.R2 => Word.repr _ 1
+                    | Model.R3 => Word.repr _ 2
+                    | Model.R4 => Word.repr _ 3
+                end). 
+Defined. 
+
+Instance foo_val : relate (Model.val) (eval_type1 val).  
+unfold relate. apply id. 
+Defined. 
+
+Instance foo_prod2 {A1 A2 B1 B2} 
+                   (H1 : relate A1 B1) 
+                   (H2 : relate A2 B2) 
+  : relate (A1*A2)%type (B1*(B2 * unit ))%type. 
+Proof. unfold relate.  intros [x y]. repeat split; auto. Defined.
+
+Instance foo_prod3 {A1 A2 A3 B1 B2 B3} 
+                  (H1 : relate A1 B1) 
+                  (H2 : relate A2 B2) 
+                  (H3 : relate A3 B3) 
+  : relate (A1*A2 * A3)%type (B1*(B2 * (B3 * unit)))%type. 
+Proof. unfold relate.  intros [[x y] z]. repeat split; auto. Defined.
+
+Instance foo_prod4 {A1 A2 A3 A4 B1 B2 B3 B4} 
+                  (H1 : relate A1 B1) 
+                  (H2 : relate A2 B2) 
+                  (H3 : relate A3 B3) 
+                  (H4 : relate A4 B4) 
+  : relate (A1*A2 * A3 * A4 )%type (B1*(B2 * (B3 * (B4 * unit))))%type. 
+Proof. unfold relate.  intros [[[u x] y] z]. repeat split; auto. Defined.
+
+Instance foo_instr : relate (Model.instr) (eval_type1 INSTR). 
+unfold relate.
+intros i. refine (match i with 
+                    | Model.loadi rd val => inl (transform (rd,val) ) 
+                    | Model.loadpc rd => inr (inl (transform rd))
+                    | Model.add r1 r2 r3 => inr (inr (inl (transform (r1,r2,r3))))
+                    | Model.bz r1 r2 => inr (inr (inr (inl (transform (r1,r2)))))
+                    | Model.load r1 r2 => inr (inr (inr (inr (inl (transform (r1,r2))))))
+                    | Model.store r1 r2 => inr (inr (inr (inr (inl (transform (r1,r2))))))
+
+                  end 
+                 ). 
+Defined. 
 
