src/TRS.v
@@ -10,7 +10,7 @@ Inductive type1 : Type :=
 
 Inductive type2 :=
   | Treg : type1 -> type2
-  | Tregfile  : Z -> type1 -> type2
+  | Tregfile  : nat -> type1 -> type2
   | Tfifo : nat -> type1 -> type2. 
 
 (** [eval_type t] computes the coq denotation of the [type] [t] *)
@@ -156,7 +156,7 @@ Section expr.
         | Eget_regfile size t v n adr => 
             let rf := get E (Tregfile size t) v ENV in 
             do adr <- eval_expr1 _ adr; 
-              @Regfile.get size _ rf  (Word.val adr)
+              @Regfile.get size _ rf  (Word.unsigned adr)
         | Efirst n t v => 
             let f := get E (Tfifo n t) v ENV in
             @FIFO.first _ n f 
@@ -169,7 +169,6 @@ Section expr.
             Some (@FIFO.isempty _  n f) 
       end. 
         
-    Require Import JMeq. 
     Fixpoint eval_expr2 t (e : expr2 t) {struct e} : eval_type2 t -> option (eval_type2 t) :=
       match e with
         | Eset t x => fun _ => eval_expr1 t x 
@@ -177,7 +176,9 @@ Section expr.
             fun old => 
               do adr <- eval_expr1 _ adr; 
               do val <- eval_expr1 t val;
-              @Regfile.set size (eval_type1 t) old (Word.val adr) val
+              let adr := Word.unsigned adr in 
+              check (lt_nat_bool adr size);
+              Some (@Regfile.set size (eval_type1 t) old adr val)
         | Epush n t x => 
             fun q => 
               do x <- eval_expr1 t x;
@@ -425,327 +426,3 @@ with
   
   Definition mk_rule' {mem} env pat cond expr : rule mem :=
     mk_rule mem env env pat (where_clause_nil _ ) cond expr. 
-
-  Module Mod. 
-  
-    Definition Num : type1 := T01 (Tint 32). 
-    Definition Val : type1 :=
-      Tunion "Val" ("MOD" of (Ttuple [Num; Num]) 
-                          :: "VAL" of (Ttuple [Num]) 
-                 :: type1_id_list_nil ). 
-    
-    Definition mod_iterate_rule : rule [Treg Val]. 
-    set (env := [Treg Num; Treg Num]). 
-    set (a := var_0 : var env (Treg Num)). 
-    set (b := var_S var_0 : var env (Treg Num)). 
-    apply (mk_rule' env). 
-
-    Definition pattern2_vector_singleton E t x :=
-      pattern2_vector_cons E _ t _ x pattern2_vector_nil. 
-    apply (pattern2_vector_singleton env). 
-    apply Plift. 
-    eapply Punion.  apply  (pattern1_disjunct_hd). 
-    apply ([| Pvar1 Num, Pvar1 Num |])%pattern. 
-    
-    apply (! b <= ! a)%expr. 
-
-      
-    Definition expr2_vector_singleton E t (x : @expr2 E t) : expr2_vector E [t] :=
-      dlist_cons t [] x (@dlist_nil type2 expr2). 
-
-    apply expr2_vector_singleton. 
-    eapply Eset. eapply Eunion. eapply expr1_disjunct_hd.  apply ([| !a - !b, !b|])%expr. 
-    Defined. 
-
-    Definition mod_done_rule : rule [Treg Val]. 
-    set (env := [Treg Num; Treg Num]). 
-    set (a := var_0 : var env (Treg Num)). 
-    set (b := var_S var_0 : var env (Treg Num)). 
-    apply (mk_rule' env). 
-    
-    apply (pattern2_vector_singleton env). 
-    apply Plift. eapply Punion. apply pattern1_disjunct_hd. 
-    apply ([| Pvar1 Num, Pvar1 Num |])%pattern. 
-    
-    apply (!a < !b)%expr. 
-    
-    apply expr2_vector_singleton. 
-    apply Eset. 
-    apply Eunion. apply expr1_disjunct_tl. apply expr1_disjunct_hd.
-    apply ([| !a |])%expr. 
-    Defined. 
-    
-    Definition TRS : TRS :=
-      {| trs_type := [Treg Val]; 
-         trs_rules := [mod_iterate_rule; mod_done_rule ]|}. 
-    
-    Definition AA : Word.T 32 := Word.repr 32 31. 
-    Definition BB : Word.T 32 := Word.repr 32 3. 
-    
-    Definition this_ENV : eval_env eval_type2 [Treg Num; Treg Num] := (AA, (BB, tt)). 
-    
-    Eval compute in run_unfair 10 TRS ((inl this_ENV, tt)). 
-    
-  End Mod. 
-
-  Module PROC. 
-    Definition val := T01 (Tint 16).
-    
-    Definition reg :=  T01 (Tint 2).  (* todo : should define an enum type *)
-    Definition RF := Tregfile 4 (val). 
-    Definition instr : type1 := 
-      Tunion "instr" ("ILOAD"  of (Ttuple [reg ;val]) 
-                   :: "LOADPC" of (reg) 
-                   :: "ADD" of (Ttuple [reg;reg;reg]) 
-                   :: "BZ" of (Ttuple [reg;reg])
-                   :: "LOAD" of (Ttuple [reg;reg])
-                   :: "STORE" of (Ttuple [reg;reg])
-                   :: type1_id_list_nil ). 
-
-    Definition IMEM := Tregfile (two_power_nat 16) instr. 
-    Definition DMEM := Tregfile (two_power_nat 16) val. 
-    Definition PC := Treg val. 
-    Definition state := [PC; RF; IMEM; DMEM]. 
-
-    Definition trivial_pattern2_vector l : pattern2_vector l l.
-    induction l. 
-    constructor. 
-    apply (pattern2_vector_cons [a] l a l). constructor.  
-    apply IHl. 
-    Defined. 
-
-    Definition WHERE E F t (p : pattern1 F t) (e : @expr1 E t) : where_clause E (E++F). 
-    eapply where_clause_cons. 
-    3: apply where_clause_nil. 
-    apply p. 
-    apply e. 
-    Defined. 
-    Arguments WHERE {E F t} p%pattern e%expr.
-
-    Notation "M  '[' ? key ']' " :=
-    (Eget_regfile _ _ M _ key)(at level 0, no associativity) : expr_scope. 
-
-    Definition IS_LOADI : pattern1 ([Treg reg ; Treg val]) instr.  
-    apply Punion. apply pattern1_disjunct_hd. apply ( [| Pvar1 reg , Pvar1 val|])%pattern. 
-    Defined. 
-
-    Definition IS_LOADPC : pattern1 ([Treg reg]) instr.  
-    apply Punion. 
-    apply pattern1_disjunct_tl. 
-    apply pattern1_disjunct_hd. apply Pvar1. 
-    Defined. 
-
-    Definition IS_ADD : pattern1 ([Treg reg; Treg reg; Treg reg]) instr.  
-    apply Punion. 
-    apply pattern1_disjunct_tl. 
-    apply pattern1_disjunct_tl. 
-    apply pattern1_disjunct_hd. apply ([| Pvar1 _ , Pvar1 _, Pvar1 _ |])%pattern. 
-    Defined. 
-
-    Definition IS_BZ : pattern1 ([Treg reg; Treg reg]) instr.  
-    apply Punion. 
-    apply pattern1_disjunct_tl. 
-    apply pattern1_disjunct_tl. 
-    apply pattern1_disjunct_tl. 
-    apply pattern1_disjunct_hd. apply ([| Pvar1 _ , Pvar1 _ |])%pattern. 
-    Defined. 
-
-    Definition IS_LOAD : pattern1 ([Treg reg; Treg reg]) instr.  
-    apply Punion. 
-    apply pattern1_disjunct_tl. 
-    apply pattern1_disjunct_tl. 
-    apply pattern1_disjunct_tl. 
-    apply pattern1_disjunct_tl. 
-    apply pattern1_disjunct_hd. apply ([| Pvar1 _ , Pvar1 _ |])%pattern. 
-    Defined. 
-
-    Definition IS_STORE : pattern1 ([Treg reg; Treg reg]) instr.  
-    apply Punion. 
-    apply pattern1_disjunct_tl. 
-    apply pattern1_disjunct_tl. 
-    apply pattern1_disjunct_tl. 
-    apply pattern1_disjunct_tl. 
-    apply pattern1_disjunct_tl. 
-    apply pattern1_disjunct_hd. apply ([| Pvar1 _ , Pvar1 _ |])%pattern. 
-    Defined. 
-
-    (* (pc,rf,imem,dmem) where LOADI(rd,const) = imem[pc]
-     –> (pc+1, rf[rd <- const], imem, dmem) *)
-    Definition loadi_rule : rule state. 
-    set (env1 := state). 
-    set (env2 := List.app state  [Treg reg ; Treg val]). 
-    set (pc := var_0 : var env1 PC). 
-    set (rf := var_S var_0 : var env1 RF). 
-    set (imem := var_S (var_S var_0) : var env1 IMEM). 
-    set (dmem := var_S (var_S (var_S var_0)) : var env1 DMEM). 
-    set (rd := var_S (var_S (var_S (var_S var_0))) : var env2 (Treg reg)). 
-    set (const := var_S (var_S (var_S (var_S (var_S var_0)))) : var env2 (Treg val)). 
-
-    apply (mk_rule state env1 env2). 
-    apply trivial_pattern2_vector. 
-    refine (WHERE IS_LOADI (imem[? !pc])%expr) . 
-      
-    apply ({< Cbool true >})%expr. 
-        
-    refine ([| Eset _ (! (var_lift  pc )+ {< Cword 1>})%expr , [!rd <- !const] , • , • |])%expr2. 
-    Defined. 
-
-
-    (* (pc,rf,imem,dmem) where LOADPC(rd) = imem[pc]
-     –> (pc+1, rf[rd <- pc], imem, dmem) *)
-
-    Definition loadpc_rule : rule state. 
-    set (env1 := state). 
-    set (env2 := List.app state  [Treg reg]). 
-    set (pc := var_0 : var env1 PC). 
-    set (rf := var_S var_0 : var env1 RF). 
-    set (imem := var_S (var_S var_0) : var env1 IMEM). 
-    set (dmem := var_S (var_S (var_S var_0)) : var env1 DMEM). 
-    set (rd := var_S (var_S (var_S (var_S var_0))) : var env2 (Treg reg)). 
-
-    apply (mk_rule state env1 env2). 
-    apply trivial_pattern2_vector. 
-    refine (WHERE IS_LOADPC (imem[? !pc])%expr) . 
-      
-    apply ({< Cbool true >})%expr. 
-        
-    refine ([| Eset _ (! (var_lift  pc )+ {< Cword 1>})%expr , [!rd <- ! (var_lift pc)] , • , • |])%expr2. 
-    Defined. 
-
-    (* (pc,rf,imem,dmem) where ADD(rd,r1,r2) = imem[pc]
-     –> (pc+1, rf[rd <- rf[r1] + rf[r2]], imem, dmem) *)
-    Definition add_rule : rule state. 
-    set (env1 := state). 
-    set (env2 := List.app state  [Treg reg; Treg reg; Treg reg]). 
-    set (pc := var_0 : var env1 PC). 
-    set (rf := var_S var_0 : var env1 RF). 
-    set (imem := var_S (var_S var_0) : var env1 IMEM). 
-    set (dmem := var_S (var_S (var_S var_0)) : var env1 DMEM). 
-    set (rd := var_S (var_S (var_S (var_S var_0))) : var env2 (Treg reg)). 
-    set (r1 := var_S (var_S (var_S (var_S (var_S var_0)))) : var env2 (Treg reg)). 
-    set (r2 := var_S (var_S (var_S (var_S (var_S (var_S var_0))))) : var env2 (Treg reg)). 
-
-    apply (mk_rule state env1 env2). 
-    apply trivial_pattern2_vector. 
-    refine (WHERE IS_ADD (imem[? !pc])%expr) . 
-      
-    apply ({< Cbool true >})%expr. 
-
-    refine ([| Eset _ (! (var_lift  pc )+ {< Cword 1>})%expr , 
-               ([!rd <- (var_lift rf)[? !r1]  + (var_lift rf)[? !r2] ])%expr 
-               , • , • |])%expr2. 
-    Defined. 
-
-
-    (* (pc,rf,imem,dmem) where BZ(rc,ra) = imem[pc] 
-     –> (rf[ra], rf , imem, dmem) when rf[rc] = 0 *)
-    Definition bztaken_rule : rule state. 
-    set (env1 := state). 
-    set (env2 := List.app state  [Treg reg; Treg reg]). 
-    set (pc := var_0 : var env1 PC). 
-    set (rf := var_S var_0 : var env1 RF). 
-    set (imem := var_S (var_S var_0) : var env1 IMEM). 
-    set (dmem := var_S (var_S (var_S var_0)) : var env1 DMEM). 
-    set (rc := var_S (var_S (var_S (var_S var_0))) : var env2 (Treg reg)). 
-    set (ra := var_S (var_S (var_S (var_S (var_S var_0)))) : var env2 (Treg reg)). 
-
-    apply (mk_rule state env1 env2). 
-    apply trivial_pattern2_vector. 
-    refine (WHERE IS_BZ (imem[? !pc])%expr) . 
-      
-    apply ( (var_lift rf) [? !rc] =  {< Cword 0 >})%expr. 
-
-    refine ([| Eset _ ((var_lift rf)[? !ra])%expr, 
-               •
-               , • , • |])%expr2. 
-    Defined. 
-
-    (* (pc,rf,imem,dmem) where BZ(rc,ra) = imem[pc] 
-     –> (pc+1, rf, imem, dmem) when rf[rc] <> 0 *)
-    Definition bznottaken_rule : rule state. 
-    set (env1 := state). 
-    set (env2 := List.app state  [Treg reg; Treg reg]). 
-    set (pc := var_0 : var env1 PC). 
-    set (rf := var_S var_0 : var env1 RF). 
-    set (imem := var_S (var_S var_0) : var env1 IMEM). 
-    set (dmem := var_S (var_S (var_S var_0)) : var env1 DMEM). 
-    set (rc := var_S (var_S (var_S (var_S var_0))) : var env2 (Treg reg)). 
-    set (ra := var_S (var_S (var_S (var_S (var_S var_0)))) : var env2 (Treg reg)). 
-
-    apply (mk_rule state env1 env2). 
-    apply trivial_pattern2_vector. 
-    refine (WHERE IS_BZ (imem[? !pc])%expr) . 
-      
-    apply ( (var_lift rf) [? !rc] <>  {< Cword 0 >})%expr. 
-
-    refine ([| Eset _ (! (var_lift  pc )+ {< Cword 1>})%expr , 
-               •
-               , • , • |])%expr2. 
-    Defined. 
-
-    (* (pc,rf,imem,dmem) where LOAD(rd,ra) = imem[pc] 
-     –> (pc+1, rf[rd := dmem[rf [ra ]]], imem, dmem) *)
-    Definition load_rule : rule state. 
-    set (env1 := state). 
-    set (env2 := List.app state  [Treg reg; Treg reg]). 
-    set (pc := var_0 : var env1 PC). 
-    set (rf := var_S var_0 : var env1 RF). 
-    set (imem := var_S (var_S var_0) : var env1 IMEM). 
-    set (dmem := var_S (var_S (var_S var_0)) : var env1 DMEM). 
-    set (rd := var_S (var_S (var_S (var_S var_0))) : var env2 (Treg reg)). 
-    set (ra := var_S (var_S (var_S (var_S (var_S var_0)))) : var env2 (Treg reg)). 
-
-    apply (mk_rule state env1 env2). 
-    apply trivial_pattern2_vector. 
-    refine (WHERE IS_LOAD (imem[? !pc])%expr) . 
-      
-    apply ({< Cbool true >})%expr. 
-
-    refine ([|Eset _ (! (var_lift  pc )+ {< Cword 1>})%expr ,
-            [ !rd <- (var_lift dmem)[? (!ra)%expr] ]
-               , • , • |])%expr2. 
-    Defined. 
-
-    (* (pc,rf,imem,dmem) where STORE(ra,r) = imem[pc] 
-     –> (pc+1, rf, imem, dmem[rf[ra] := rf[r]]) *)
-    Definition store_rule : rule state. 
-    set (env1 := state). 
-    set (env2 := List.app state  [Treg reg; Treg reg]). 
-    set (pc := var_0 : var env1 PC). 
-    set (rf := var_S var_0 : var env1 RF). 
-    set (imem := var_S (var_S var_0) : var env1 IMEM). 
-    set (dmem := var_S (var_S (var_S var_0)) : var env1 DMEM). 
-    set (ra := var_S (var_S (var_S (var_S var_0))) : var env2 (Treg reg)). 
-    set (r := var_S (var_S (var_S (var_S (var_S var_0)))) : var env2 (Treg reg)). 
-
-    apply (mk_rule state env1 env2). 
-    apply trivial_pattern2_vector. 
-    refine (WHERE IS_STORE (imem[? !pc])%expr) . 
-      
-    apply ({< Cbool true >})%expr. 
-
-    refine ([|Eset _ (! (var_lift  pc )+ {< Cword 1>})%expr ,
-            •,
-            • , [(var_lift rf)[? (!ra)%expr] <- (var_lift rf) [?(!r)%expr]] |])%expr2. 
-    Defined. 
-
-    
-    Definition TRS : TRS :=
-      {| trs_type := state; 
-         trs_rules := [ 
-                       loadi_rule;
-                       loadpc_rule;
-                       add_rule;
-                       bztaken_rule;
-                       bznottaken_rule;
-                       load_rule;
-                       store_rule
-                      ]|}. 
-    
-    Definition init : eval_env eval_type2 state.
-    unfold eval_env. red. 
-    split. simpl. apply (Word.repr _ 0). 
-    split. simpl. apply Regfile.empty. apply (Word.repr _ 0).
-    split. simpl eval_env. compute. 
-    Admitted. 
-  End PROC. 
