src/Vector.v
@@ -1,0 +1,189 @@
+
+(** Vectors: n-uples *)
+Require List. 
+Section t. 
+  Variable t : Type. 
+  Fixpoint vector n : Type := match n with 
+                         | 0 => unit
+                         | S n => (t * vector n)%type
+                       end.
+
+  Definition nil : vector 0 := tt. 
+  Definition cons {n} x (v : vector n) : vector (S n) := 
+    (x,v).
+
+  Fixpoint get n : vector n -> nat ->  option t :=
+    match n with 
+      | 0 => fun _ _ => None
+      | S n => fun v x => match x with 
+                              | 0 => Some (fst v)
+                              | S x => get n (snd v) x
+                          end
+    end.
+
+  (* silently fails to update out of bounds values *)
+  Fixpoint set n : vector n -> nat -> t -> vector n :=
+    match n with 
+      | 0 => fun v _ _ => v
+      | S n => fun v x el => match x with 
+                              | 0 => (el, snd v)
+                              | S x => (fst v, set n (snd v) x el)
+                          end
+    end.
+
+  Fixpoint empty n x : vector n :=
+    match n with 
+        | 0 => nil
+        | S n => cons x (empty n x)
+    end. 
+
+  Fixpoint of_list (l : list t) : vector (List.length l) :=
+    match l with 
+      | List.nil => nil
+      | List.cons t q => cons t (of_list q)
+    end. 
+
+  Fixpoint of_list_pad n (el : t) (l : list t) : vector n :=
+    match n with 
+        | 0 => nil
+        | S p => match l with 
+                  | List.nil => empty (S p) el
+                  | List.cons t q => cons t (of_list_pad p el q)
+                end
+    end. 
+
+End t. 
+
+Section eq. 
+  Context {A : Type} (eq : A -> A -> bool).
+  Fixpoint veqb n  : vector A n -> vector A n -> bool :=
+    match n with 
+      0 => fun l l' => true
+      | S n => fun l l' => 
+        match l,l' with
+          | (x,q), (x',q') => andb (eq x x') (veqb n q q')
+        end
+    end.
+End eq. 
+
+Arguments Scope vector [type_scope nat_scope]. 
+Definition uncons {A} n (v : vector A (S n)) : A * vector A n := id v.
+Lemma nil_eq {A} (u v : vector A 0) : u = v. 
+Proof. 
+  destruct u. destruct v. reflexivity. 
+Qed.
+
+Section map. 
+  Context{ A B : Type} ( f : A -> B).
+  Fixpoint map n : vector A n -> vector B n := match n with 
+                      | 0 => fun _ => tt
+                      | S p => fun v => 
+                        match v with 
+                          |(t,q) => (f t, map p q)
+                        end
+                    end.
+End map. 
+Section ops.
+  Context {A B : Type}.
+
+  Fixpoint vector_repeat n (x :A ) : vector A n :=
+    match n with 
+      | 0 => tt
+      | S p => (x, vector_repeat p x)
+    end. 
+    
+  Fixpoint last n x : vector A n -> A :=
+    match n with 
+      | 0 => fun _ => x 
+      | S p => fun v => 
+        match v with | (t,q) => last p t q end 
+    end.
+  
+  Definition forget_right n (v : vector (A *B) n) : vector A n :=
+  map (@fst A B) n v.
+
+  Definition forget_left n (v : vector (A *B) n) : vector B n :=
+    map (@snd A B) n v.
+
+  Definition unzip n (v : vector (A *B) n) : vector A n * vector B n :=
+     (forget_right n v , forget_left n v).
+  
+  Fixpoint zip n : 
+    vector A n -> vector B n -> vector (A*B) n :=
+    match n with 
+      0 => fun _ _ => tt
+      | S p => 
+        fun v v' =>
+          match v,v' with 
+            | (t,q),(t',q') => ((t,t'), (zip p q q'))
+          end
+    end.
+    
+  Fixpoint append n m : vector A n ->  vector A m -> vector A (n +m) :=
+  match n with 
+    | 0 => fun u v => v
+    | S p => 
+      fun u v => 
+        match u with 
+          (t,q) => (t,append p m q v)
+        end
+  end.
+
+  Fixpoint firstn  n m: vector A (n + m) -> vector A n :=
+    match n with 
+      | 0 => fun v => tt
+      | S p => fun v => match v with 
+                        | (t,q) => (t,firstn p m q)
+                      end
+    end.
+
+  Fixpoint skipn  n m: vector A (n + m) -> vector A m :=
+    match n with 
+      | 0 => fun v => v
+      | S p => fun v => match v with 
+                        | (t,q) => (skipn p m q)
+                      end
+    end.
+
+End ops. 
+
+Section pointwise. 
+  Context {A B : Type}.
+  Context (R : A -> B -> Prop).
+  
+  Fixpoint pointwise n : vector A n -> vector B n -> Prop :=
+    match n with 
+      | 0 => fun _ _  => True
+      | S p => fun u => fun v => 
+        match u,v with 
+          (t,q),(t',q') => R t t' /\ pointwise p q q'
+        end
+    end. 
+End pointwise. 
+
+Section pairmap.
+  Context {A B : Type}.
+  Variable f : A -> A -> B. 
+
+  Fixpoint pairmap n x : vector A n -> vector B n :=
+    match n with 
+      | 0 => fun v => tt
+      | S p => fun v => match v with 
+                        | (t,q) => (f t x,pairmap p t q)
+                      end
+    end.
+  Lemma pairmap_append x n m (s1 : vector A n) (s2 : vector A m) :
+    pairmap (n + m) x (append n m s1 s2) = 
+    append n m (pairmap n x s1) (pairmap m (last n x s1) s2).
+  Proof. 
+    revert x. 
+    induction n; intros x.  simpl. reflexivity. 
+    simpl in s1. destruct s1 as [t q].    
+    simpl.
+    rewrite IHn. 
+    reflexivity. 
+  Qed.
+End pairmap. 
+
+  
+
